some refactoring, added an ODH module

examples/rel/Setoids.Crypto.fst
@@ -1,10 +1,11 @@
 module Setoids.Crypto
 module L = Setoids
 open FStar.Bytes
+open FStar.UInt32
 open FStar.Map
 open Setoids
 
-module DMap = FStar.DependentMap
+module DM = FStar.DependentMap
 
 //let byte = uint_8
 
@@ -21,24 +22,17 @@ module DMap = FStar.DependentMap
 ///      making it unavailable for reasoning.
 ///
 ///      Maybe we'll revise it
-let tape = nat -> Tot byte
-let index = nat
+let tape = u32 -> Tot byte
+let index = u32
 
 let default_tape_rel = lo tape
 let default_index_rel = lo index
 
-let truncate (t:tape) (n:index) : tape =
-  fun m -> t (m + n)
-
-/// The type of effectful computations with 3 effects
-///    1. random sampling
-///    2. reading and writing state
-///    3. raising exceptions
-//let eff (st:Type) (a:Type) =
-//  tape & st ->  //input tape and initial state
-//  Tot (option a &  //normal return (Some _) or exception (None)
-//       st &        //final state
-//       nat)          //amount of tape consumed
+//#set-options "--z3rlimit 150 --max_fuel 1 --max_ifuel 2 --query_stats"
+#set-options "--z3rlimit 150 --query_stats"
+let truncate (t:tape) (n:u32) : tape =
+  fun m ->
+    t (add_underspec m n)
 
 let option_rel (#a:Type) (arel:rel a) =
   fun (x:option a) (y:option a) ->
@@ -95,26 +89,9 @@ let eff_rel #s #a
 /// returning a result into a computation
 let return (#s:Type) (#a:Type) (#srel:erel s) (#arel:erel a) (x:a)
   : eff #s #a srel arel
-  = fun ((t:tape), (s0:s)) -> Some x, s0, 0
+  = fun ((t:tape), (s0:s)) -> Some x, s0, 0ul
 
 /// sequential composition of `eff` computations
-//let bind #st #a #b
-//         (f:eff st a)
-//         (g: a -> eff st b)
-//  : eff st b
-//  = fun (t, s) ->
-//       match f (t, s) with
-//       | None, s', n ->
-//         // if f raises an exception, propagate it, while preserving
-//         // the state (s') and #slots consumed on the tape (n)
-//         None, s', n
-//
-//       | Some v, s', n ->
-//         //otherwise, truncate the prefix of the tape that was already
-//         //used (n) and call `g` with the result of `f`, the truncated
-//         //tape and the state produced by `f` (s')
-//         g v (truncate t n, s')
-//#set-options "--z3rlimit 350 --max_fuel 1 --max_ifuel 3"
 #set-options "--z3rlimit 150 --max_fuel 1 --max_ifuel 2"
 let bind #s #a (#srel:erel s) (#arel:erel a) #b (#brel:erel b)
          ($f:eff #s #a srel arel)
@@ -127,280 +104,64 @@ let bind #s #a (#srel:erel s) (#arel:erel a) #b (#brel:erel b)
      | None, s1, n ->
        None, s1, n
 
+#set-options "--z3rlimit 150 --max_fuel 1 --max_ifuel 2 --query_stats"
 /// reading the entire state
 let get #s (#srel:erel s) : eff srel srel =
-  fun (t, s0) -> Some s0, s0, 0
+  fun (t, s0) -> Some s0, s0, 0ul
 
 /// writing the entire state
 let put #s (#srel:erel s) : (srel ^--> eff_rel srel (lo unit)) =
-  fun s (t,_) -> Some (), s, 0
+  fun s (t,_) -> Some (), s, 0ul
 
 /// sampling from the head of the tape
 let sample #st : eff st (lo byte)
-  = fun (t, s) -> Some (t 0), s, 1
+  = fun (t, s) -> Some (t 0ul), s, 1ul
 
-let sample_multiple #s #srel (length:nat) :eff srel (lo (lbytes length)) =
+let rec sample_inner (t:u32 -> byte) (c:u32) : Tot (lbytes32 c) (decreases (v c)) =
+  match c with
+  | 0ul -> empty_bytes
+  | c' ->
+    let b = t (sub c 1ul) in
+    let rest = sample_inner t (sub c 1ul) in
+    append rest (create 1ul b)
+
+let sample_multiple #s #srel (length:u32) :eff #s srel (lo (lbytes32 length)) =
   fun (t, s) ->
-  let rec sample_inner c =
-    match c with
-    | 0 -> empty_bytes
-    | c' ->
-      let b = t (c - 1) in
-      let rest = sample_inner (c - 1) in
-      append rest (create 1ul b)
-  in
-  let b_string = sample_inner length in
+  let b_string = sample_inner t length in
   Some b_string, s, length
 
-
-//let sample_multiple #s #srel (length:nat) :eff srel (lo (lbytes length))=
-//  let rec sample_inner #s #srel (c:nat{c < length}) : eff #s #(lbytes (length - c)) srel (lo (lbytes (length - c))) =
-//    match c with
-//    | 0 -> return #s #(lbytes 0) #srel #(lo (lbytes 0)) empty_bytes
-//    | c' ->
-//      b <-- sample;
-//      rest <-- sample_inner #s #srel (c - 1);
-//      return (append (create 1ul b) rest)
-//  in
-//  b_string <-- sample_inner length;
-//  return #s #(lbytes length) #srel #(lo (lbytes length)) b_string
-
-
-
-
-(* Old effect *)
 /// raising an exception
 let raise #s (#srel:erel s) #a (#arel:erel a) : eff srel arel
-  = fun (t, s) -> (None, s, t)
+  = fun (t, s) -> (None, s, 0ul)
 
-#set-options "--z3rlimit 350 --max_fuel 3 --max_ifuel 4"
+#reset-options
+#set-options "--z3rlimit 350 --query_stats --max_fuel 4 --max_ifuel 5"
 /// state separation
-let lift_left #s1 (#s1rel:erel s1) #s2 (#s2rel:erel s2) #a (#arel:erel a) (f:(default_tape_rel ** s1rel) ^--> (triple_rel (option_rel arel) s1rel default_tape_rel))
-  : ((default_tape_rel ** (s1rel **s2rel)) ^--> (triple_rel (option_rel arel) (s1rel ** s2rel) default_tape_rel))
+let lift_left (#s1:Type) (#s1rel:erel s1{lo s1 == s1rel}) #s2 (#s2rel:erel s2) #a (#arel:erel a) ($f:(default_tape_rel ** s1rel) ^--> (triple_rel (option_rel arel) (lo int) (lo index)))
+  : ((default_tape_rel ** (s1rel ** s2rel)) ^--> (triple_rel (option_rel arel) (lo int ** s2rel) (lo index)))
   = fun (t, (s1, s2)) ->
-      match f (t, s1) with
-      | None, s1', t ->
-        None, (s1', s2), t
+      match f (t ,s1) with
+      | None, s1', n ->
+        None, (s1', s2), n
 
-      | Some x, s1', t ->
-        Some x, (s1', s2), t
+      | Some x, s1', n ->
+        Some x, (s1', s2), n
 
-let lift_right #s1 (#s1rel:erel s1) #s2 (#s2rel:erel s2) #a (#arel:erel a) (f:eff s2rel arel)
+let lift_right #s1 (#s1rel:erel s1) #s2 (#s2rel:erel s2{s2rel == lo s2}) #a (#arel:erel a) (f:eff s2rel arel)
   : eff (s1rel ** s2rel) arel
   = fun (t, (s1, s2)) ->
       match f (t, s2) with
       | None, s2', t -> None, (s1, s2'), t
       | Some x, s2', t -> Some x, (s1, s2'), t
 
-module DM = FStar.DependentMap
-
-////////////////////////////////////////////////////////////////////////////////
-//KEY package
-////////////////////////////////////////////////////////////////////////////////
-
-let lbytes (n:nat) = Seq.lseq byte n
-let bytes = Seq.seq byte
-let handle = bytes&bytes
-let key (n:nat) = lbytes n
-let key_state (n:nat) = (Map.t handle (option bool) & Map.t handle (option (key n)))
-
-let key_state_rel (n:nat) = lo (key_state n)
-
-let key_eff (n:nat) = eff (key_state_rel n)
-
-//let key_gen (h:handle) : eff (key_state 1) handle =
-//    s <-- get ;
-//    let (h_map,k_map) = s in
-//    match Map.contains h_map h,Map.contains k_map h with
-//    | false,false ->
-//      k <-- sample ;
-//      let s':key_state 1 = (Map.upd h_map h true, Map.upd k_map h (Seq.create 1 k <: Seq.lseq byte 1)) in
-//      set s' ;;
-//      return h
-//    | _,_ ->
-//      raise
-//
-
-let key_set_t (n:nat) = (lo handle) ** (lo (Seq.lseq byte n)) ^--> eff_rel (key_state_rel n) (lo handle)
-let key_set n : key_set_t n =
-    fun (h, k_in) ->
-    s <-- get ;
-    let (h_map,k_map) = s in
-    match Map.sel h_map h,Map.sel k_map h with
-    | None,None ->
-      let s':key_state n = (Map.upd h_map h (Some true), Map.upd k_map h (Some k_in)) in
-      put s' ;;
-      return h
-    | _,_ ->
-      raise
-
-let key_cset_t (n:nat) = (lo handle) ** (lo (Seq.lseq byte n)) ^--> eff_rel (key_state_rel n) (lo handle)
-let key_cset n : key_cset_t n =
-    fun (h, k_in) ->
-    s <-- get ;
-    let (h_map,k_map) = s in
-    match Map.sel h_map h,Map.sel k_map h with
-    | None, None ->
-      let s':key_state n = (Map.upd h_map h (Some false), Map.upd k_map h (Some k_in)) in
-      put s' ;;
-      return h
-    | _,_ ->
-      raise
-
-let key_get_t (n:nat) = (lo handle) ^--> eff_rel (key_state_rel n) (lo (key n))
-let key_get n : key_get_t n =
-    fun h ->
-    s <-- get ;
-    let (h_map,k_map) = s in
-    match Map.sel h_map h,Map.sel k_map h with
-    | Some hon, Some k ->
-      return k
-    | _,_ ->
-      raise
-
-let transform n (h:handle) = key_get n h
-
-
-let key_hon_t (n:nat) = (lo handle) ^--> eff_rel (key_state_rel n) (lo bool)
-let key_hon n : key_hon_t n =
-    fun h ->
-    s <-- get ;
-    let (h_map,k_map) = s in
-    match Map.sel h_map h,Map.sel k_map h with
-    | Some hon, Some k ->
-      return hon
-    | _,_ ->
-      raise
-
-type key_labels =
-    | GET
-    | HON
-    | SET
-    | CSET
-
-let key_field_types n : key_labels -> Type =
-    function  GET -> key_get_t n
-            | HON -> key_hon_t n
-            | SET -> key_set_t n
-            | CSET -> key_cset_t n
-
-let key_field_rels n : (k:key_labels -> erel (key_field_types n k)) =
-  function
-      GET -> arrow (lo handle) (eff_rel (key_state_rel n) (lo (key n)))
-    | HON -> arrow (lo handle) (eff_rel (key_state_rel n) (lo bool))
-    | SET -> arrow (lo handle**lo (lbytes n)) (eff_rel (key_state_rel n) (lo handle))
-    | CSET -> arrow (lo handle**lo (lbytes n)) (eff_rel (key_state_rel n) (lo handle))
-
-let sig_key (n:nat) = {
-  labels = key_labels;
-  ops = key_field_types n;
-  rels = key_field_rels n
-  }
-
-let key_module (n:nat) : module_t (sig_key n) =
-  DM.create #_ #(sig_key n).ops
-    (function GET -> key_get n
-            | HON -> key_hon n
-            | SET -> key_set n
-            | CSET -> key_cset n)
-
-let key_functor n = as_fun (key_module n)
-
-////////////////////////////////////////////////////////////////////////////////
-//AE package
-////////////////////////////////////////////////////////////////////////////////
-noeq type ae_scheme (n:nat) =
-  | AES:
-  max_plaintext_length: u32 ->
-  ciphertext_length: (plaintext_length:u32{plaintext_length `lte` max_plaintext_length} -> u32) ->
-  enc: (p:bytes -> k:key n -> nonce:bytes -> c:bytes) ->
-  dec: (c:bytes -> k:key n -> nonce:bytes -> option (p:bytes)) ->
-  ae_scheme n
-
-/// Map from nonces to a maps from ciphertext to plaintexts
-let ae_log #n (aes:ae_scheme n) =
-  DM.t bytes (fun n -> option (DM.t bytes (fun i -> option bytes)))
-
-let ae_log_rel (#n:nat) (aes:ae_scheme n) = lo (ae_log aes)
-
-/// Is there a nicer way to have a function with mulitple inputs than using nested tuples?
-/// How to use the 'secure information flow' relations again with AE^0 vs AE^1?
-/// AE^0 also depends on the state of the key package.
-/// Is there a way to improve verification performance and/or error messages?
-/// Every AE function takes as additional parameter the module it is composed with.
-/// AE Functor: Function from underlay module to AE signature
-
-let enc_inputs (#a:Type) (#b:Type) (#c:Type) (arel:rel a) (brel:rel b) (crel: rel c) (p0 p1:(a & b & c)) : prop =
-  let (w0, x0, y0) = p0 in
-  let (w1, x1, y1) = p1 in
-  w0 `arel` w1 /\
-  x0 `brel` x1 /\
-  y0 `crel` y1 ///\
-  //z0 `drel` z1
-
-#set-options "--z3rlimit 50 --max_fuel 1 --max_ifuel 3"
-/// This would be a nice, generic approach, but it's probably a little to complex
-//let multi_rel' (tl:list Type) (rm:DMap.t (n:nat{n < List.Tot.length tl}) (fun i -> rel (List.Tot.index tl i))) (vm0 vm1:DMap.t (n:nat{n < List.Tot.length tl}) (fun i -> List.Tot.index tl i)) =
-//  let logical_and t1 t2 = t1 /\ t2
-//  let iterate_maps (i:nat{i < List.Tot.length tl}) =
-//    let x0 = DMap.sel vm0 i in
-//    let x1 = DMap.sel vm1 i in
-//    let rel = DMap.sel rm i in
-//    x0 `rel` x1
-//  in
-//  //let indices = mapi #Type (fun i _ -> i) tl in
-//  let prop_list = List.Tot.mapi #Type (fun i _ -> iterate_maps i) tl in
-//  admit()
-
-/// TODO: Find a way to improve this such that it can take more arguments and call the function directly.
 let get_oracle #sig (m:module_t sig) (o:sig.labels) : sig.ops o = DM.sel m o
 
-#set-options "--z3rlimit 350 --max_fuel 2 --max_ifuel 3"
-let enc_0_t (n:nat) (aes:ae_scheme n) = enc_inputs (lo bytes) (lo bytes) (lo handle) ^--> eff_rel (ae_log_rel #n aes ** lo (key_state n)) (lo bytes)
-let enc_1_t (n:nat) (aes:ae_scheme n) = enc_inputs (lo bytes) (lo bytes) (lo handle) ^--> eff_rel (ae_log_rel #n aes ** hi (key_state n)) (lo bytes)
-
-let enc_0 (n:nat) (aes:ae_scheme n) (key_module:module_t (sig_key n)) : (enc_0_t n aes) = // (#n:nat) (key_module:module_t (sig_key n)) (aes:ae_scheme n) (inputs:enc_inputs (lo bytes) (lo bytes) (lo handle)) : (eff (lo (ae_state #n aes)) (lo bytes)) =
-  fun ((p:bytes),(nonce:bytes),(h:handle)) ->
-  ae_st <-- get ;
-  let ae_st,k_st = ae_st in
-  match DM.sel ae_st nonce with
-  | Some option_map ->
-    raise
-  | None ->
-    let k_get : key_get_t n = get_oracle key_module GET in
-    k <-- lift_right #(ae_log #n aes) #(ae_log_rel #n aes) #(key_state n) #(key_state_rel n) #(key n) #(lo (key n)) (k_get h);
-    let c = aes.enc p k nonce in
-    return c
-
-let enc_1 (n:nat) (aes:ae_scheme n) (key_module:module_t (sig_key n)) : (enc_0_t n aes) = // (#n:nat) (key_module:module_t (sig_key n)) (aes:ae_scheme n) (inputs:enc_inputs (lo bytes) (lo bytes) (lo handle)) : (eff (lo (ae_state #n aes)) (lo bytes)) =
-  fun ((p:bytes),(nonce:bytes),(h:handle)) ->
-  ae_st <-- get ;
-  let ae_st,k_st = ae_st in
-  match DM.sel ae_st nonce with
-  | Some option_map ->
-    raise
-  | None ->
-    let k_get : key_get_t n = get_oracle key_module GET in
-    k <-- lift_right #(ae_log #n aes) #(ae_log_rel #n aes) #(key_state n) #(key_state_rel n) #(key n) #(lo (key n)) (k_get h);
-    let c = aes.enc p k nonce in
-    return c
-
-// ////////////////////////////////////////////////////////////////////////////////
-// //ODH package
-// ////////////////////////////////////////////////////////////////////////////////
-
-// let share (n:nat) = lbytes n
-// let exponent (n:nat) = lbytes n
-// assume val exponentiate : #n:nat -> x:share n -> y:exponent n -> share
-// let odh
-
-// let odh_0  : (eff (ae_key_state aes) bytes) =
-//   state <-- get ;
-//   let ae_st = fst state in
-//   let key_st = snd state in
-//   match Map.contains ae_st nonce with
-//   | true ->
-//     raise
-//   | false ->
-//     let c = Map.upd ae_st nonce (Map.sel ae_st plain) in
-//     return c
+/// Problems until now:
+/// - can't prove lift_left and lift_right without requiring one of the state
+///   relations to be 'lo'.
+/// - can't prove that ae0_functor is actually a functor. I suspect this is
+///   somehow because the 'lo' effect on the key module state.
+/// - if two parallely composed packages have the same underlay, they should not
+///   require two instance of this signature, which is what functor_prod gives you.
+///   - a question on the implementation of sig_prod. What if the signatures are
+///     the same? Then does the call always go to the first one?
