examples/rel/Setoids.Crypto.AE.fst
@@ -1,0 +1,220 @@
+module Setoids.Crypto.AE
+open FStar.Bytes
+open FStar.UInt32
+open FStar.Map
+open Setoids
+open Setoids.Crypto
+open Setoids.Crypto.KEY
+
+module DM = FStar.DependentMap
+
+////////////////////////////////////////////////////////////////////////////////
+//AE package
+////////////////////////////////////////////////////////////////////////////////
+
+noeq type ae_scheme (n:u32) =
+  | AES:
+  max_plaintext_length: u32 ->
+  ciphertext_length: (plaintext_length:u32{plaintext_length `lte` max_plaintext_length} -> u32) ->
+  enc: (p:bytes -> k:key n -> nonce:bytes -> c:bytes) ->
+  dec: (c:bytes -> k:key n -> nonce:bytes -> option (p:bytes{len p `lte` max_plaintext_length})) ->
+  ae_scheme n
+
+let ae_log_key = handle*bytes
+let ae_log_value #n (aes:ae_scheme n) = fun (h,nonce) -> option (bytes*p:bytes{len p `lte` aes.max_plaintext_length})
+
+/// Map from nonces to a maps from ciphertext to plaintexts
+let ae_log #n (aes:ae_scheme n) =
+  DM.t (handle*bytes) (ae_log_value aes)
+
+let ae_log_rel (#n:u32) (aes:ae_scheme n) = lo (ae_log aes)
+
+let combined_state_t #n aes = ae_log #n aes * key_state n
+
+/// Is there a nicer way to have a function with mulitple inputs than using nested tuples?
+/// How to use the 'secure information flow' relations again with AE^0 vs AE^1?
+/// AE^0 also depends on the state of the key package.
+/// Is there a way to improve verification performance and/or error messages?
+/// Every AE function takes as additional parameter the module it is composed with.
+/// AE Functor: Function from underlay module to AE sigu32ure
+
+#set-options "--z3rlimit 50 --max_fuel 1 --max_ifuel 3"
+/// This would be a nice, generic approach, but it's probably a little to complex
+//let multi_rel' (tl:list Type) (rm:DMap.t (n:u32{n < List.Tot.length tl}) (fun i -> rel (List.Tot.index tl i))) (vm0 vm1:DMap.t (n:u32{n < List.Tot.length tl}) (fun i -> List.Tot.index tl i)) =
+//  let logical_and t1 t2 = t1 /\ t2
+//  let iterate_maps (i:u32{i < List.Tot.length tl}) =
+//    let x0 = DMap.sel vm0 i in
+//    let x1 = DMap.sel vm1 i in
+//    let rel = DMap.sel rm i in
+//    x0 `rel` x1
+//  in
+//  //let indices = mapi #Type (fun i _ -> i) tl in
+//  let prop_list = List.Tot.mapi #Type (fun i _ -> iterate_maps i) tl in
+//  admit()
+
+let enc_inputs #n (aes:ae_scheme n) = triple_rel (lo (p:bytes{len p `lte` aes.max_plaintext_length})) (lo bytes) (lo handle)
+
+#set-options "--z3rlimit 350 --max_fuel 2 --max_ifuel 3"
+let enc_0_t (n:u32) (aes:ae_scheme n) =
+  enc_inputs aes
+    ^--> eff_rel (ae_log_rel #n aes ** lo (key_state n)) (lo bytes)
+let enc_1_t (n:u32) (aes:ae_scheme n) =
+  enc_inputs aes
+    ^--> eff_rel (ae_log_rel #n aes ** hi (key_state n)) (lo bytes)
+
+let enc_0 (n:u32) (aes:ae_scheme n) (key_module:module_t (key_sig n)) : (enc_0_t n aes) =
+  fun (p,nonce,h) ->
+    combined_state <-- get ;
+    let ae_st,k_st = combined_state in
+    match DM.sel #ae_log_key #(ae_log_value aes) ae_st (h,nonce) with
+    | Some option_map ->
+      raise #(ae_log #n aes*key_state n)
+    | None ->
+      let k_get : key_get_t n = get_oracle key_module GET in
+      k <-- lift_right #(ae_log #n aes) #(ae_log_rel #n aes) #(key_state n) #(key_state_rel n) #(key n) #(lo (key n)) (k_get h);
+      let c = aes.enc p k nonce in
+      let ae_st' = DM.upd ae_st (h,nonce) (Some (c,p)) in
+      put (ae_st',k_st);;
+      return c
+
+
+#reset-options
+#set-options "--z3rlimit 350 --max_fuel 2 --max_ifuel 3"
+#set-options "--query_stats"
+let enc_1 (n:u32) (aes:ae_scheme n) (key_module:module_t (key_sig n)) : (enc_1_t n aes) =
+  fun (p,nonce,h) ->
+    combined_state <-- get ;
+    let ae_st,k_st : ae_log aes*key_state n = combined_state in
+    match DM.sel #ae_log_key #(ae_log_value aes) ae_st (h,nonce) with
+    | Some option_map -> // Nonce is not unique
+      raise
+    | None ->
+      c <-- sample_multiple (aes.ciphertext_length (len p));
+      let ae_st' = DM.upd ae_st (h,nonce) (Some (c,p)) in
+      put (ae_st',k_st);;
+      return #(ae_log #n aes*key_state n) #(bytes) #(ae_log_rel #n aes ** key_state_rel n) #(lo bytes) c
+
+let dec_inputs #n (aes:ae_scheme n) = triple_rel (lo (c:bytes{len c `lte` aes.ciphertext_length aes.max_plaintext_length})) (lo bytes) (lo handle)
+
+let dec_0_t (n:u32) (aes:ae_scheme n) =
+  dec_inputs aes
+  ^--> eff_rel (ae_log_rel #n aes ** lo (key_state n)) (lo (option (p:bytes{len p `lte` aes.max_plaintext_length})))
+let dec_1_t (n:u32) (aes:ae_scheme n) =
+  dec_inputs aes
+    ^--> eff_rel (ae_log_rel #n aes ** hi (key_state n)) (lo (option (p:bytes{len p `lte` aes.max_plaintext_length})))
+
+let dec_0 (n:u32) (aes:ae_scheme n) (key_module:module_t (key_sig n)) : (dec_0_t n aes) =
+  fun (c,nonce,h) ->
+  combined_state <-- get ;
+  let ae_st,k_st = combined_state in
+  let k_get : key_get_t n = get_oracle key_module GET in
+  k <-- lift_right #(ae_log #n aes) #(ae_log_rel #n aes) #(key_state n) #(key_state_rel n) #(key n) #(lo (key n)) (k_get h);
+  return (aes.dec c k nonce)
+
+let dec_1 (n:u32) (aes:ae_scheme n) (key_module:module_t (key_sig n)) : (dec_1_t n aes) =
+  fun (c,nonce,h) ->
+  combined_state <-- get ;
+  let ae_st,k_st : ae_log aes*key_state n = combined_state in
+  match DM.sel ae_st (h,nonce) with
+  | Some (c',p) -> // Nonce is not unique
+    if c = c' then
+      return #(combined_state_t #n aes) (Some p)
+    else
+      return None
+  | None ->
+    return #(combined_state_t #n aes) #_ #(ae_log_rel #n aes ** hi (key_state n)) #(lo (option (p:bytes{len p `lte` aes.max_plaintext_length}))) None
+
+type ae_labels =
+    | ENC
+    | DEC
+
+let ae0_field_types n aes : ae_labels -> Type =
+    function  ENC -> enc_0_t n aes
+            | DEC -> dec_0_t n aes
+
+let ae1_field_types n aes : ae_labels -> Type =
+    function  ENC -> enc_1_t n aes
+            | DEC -> dec_1_t n aes
+
+let ae0_field_rels n aes : (l:ae_labels -> erel (ae0_field_types n aes l)) =
+  function
+      ENC -> arrow (enc_inputs aes) (eff_rel (ae_log_rel #n aes ** lo (key_state n)) (lo bytes))
+    | DEC -> arrow (dec_inputs aes) (eff_rel (ae_log_rel #n aes ** lo (key_state n)) (lo (option (p:bytes{len p `lte` aes.max_plaintext_length}))))
+
+let ae1_field_rels n aes : (l:ae_labels -> erel (ae1_field_types n aes l)) =
+  function
+      ENC -> arrow (enc_inputs aes) (eff_rel (ae_log_rel #n aes ** hi (key_state n)) (lo bytes))
+    | DEC -> arrow (dec_inputs aes) (eff_rel (ae_log_rel #n aes ** hi (key_state n)) (lo (option (p:bytes{len p `lte` aes.max_plaintext_length}))))
+
+let sig_ae0 (n:u32) (aes:ae_scheme n) = {
+  labels = ae_labels;
+  ops = ae0_field_types n aes;
+  rels = ae0_field_rels n aes
+  }
+
+let sig_ae1 (n:u32) (aes:ae_scheme n) = {
+  labels = ae_labels;
+  ops = ae1_field_types n aes;
+  rels = ae1_field_rels n aes
+  }
+
+let ae0_module (n:u32) (aes:ae_scheme n) (k:module_t (key_sig n)) : module_t (sig_ae0 n aes) =
+  DM.create #_ #(sig_ae0 n aes).ops
+    (function ENC -> enc_0 n aes k
+            | DEC -> dec_0 n aes k)
+
+let ae1_module (n:u32) (aes:ae_scheme n) (k:module_t (key_sig n)) : module_t (sig_ae1 n aes) =
+  DM.create #_ #(sig_ae1 n aes).ops
+    (function ENC -> enc_1 n aes k
+            | DEC -> dec_1 n aes k)
+
+/// This doesn't cast to a functor properly
+let ae0_functor (n:u32) (aes:ae_scheme n)
+  //: functor_t (key_sig n) (sig_ae0 n aes)
+  = fun (k:module_t (key_sig n)) -> ae0_module n aes k
+
+let ae1_functor (n:u32) (aes:ae_scheme n)
+  : functor_t (key_sig n) (sig_ae1 n aes)
+  = fun (k:module_t (key_sig n)) -> ae1_module n aes k
+
+type id_ae_labels =
+  | ID_SET
+  | ID_CSET
+
+let id_ae_field_types n : id_ae_labels -> Type0 =
+    function ID_SET -> key_set_t n
+           | ID_CSET -> key_cset_t n
+
+let id_ae_field_rels n : (l:id_ae_labels -> erel (id_ae_field_types n l)) =
+  function ID_SET -> arrow (lo handle ** lo (key n)) (eff_rel (key_state_rel n) (lo handle))
+         | ID_CSET -> arrow (lo handle ** lo (key n)) (eff_rel (key_state_rel n) (lo handle))
+
+let sig_id_ae (n:u32) = {
+  labels = id_ae_labels;
+  ops = id_ae_field_types n;
+  rels = id_ae_field_rels n
+  }
+
+#set-options "--z3rlimit 350 --max_fuel 3 --max_ifuel 4"
+let id_ae_module (n:u32) (km:module_t (key_sig n)) : module_t (sig_id_ae n) =
+  DM.create #_ #(sig_id_ae n).ops
+    (function ID_SET -> get_oracle km SET
+            | ID_CSET -> get_oracle km CSET)
+
+let id_ae_functor n
+  : functor_t (key_sig n) (sig_id_ae n)
+  = fun (k:module_t (key_sig n)) -> id_ae_module n k
+
+//let ae_game0 n (aes:ae_scheme n) (km:module_t (key_sig n)) =
+//  functor_prod
+//    (key_sig n) (sig_id_gen n)
+//    (key_sig n) (sig_ae0 n aes)
+//    (id_ae_functor n)
+//    (ae0_functor n aes)
+
+let ae_game1 n (aes:ae_scheme n) (km:module_t (key_sig n)) =
+  functor_prod
+    (key_sig n) (sig_id_ae n)
+    (key_sig n) (sig_ae1 n aes)
+    (id_ae_functor n)
+    (ae1_functor n aes)
