examples/rel/Setoids.Crypto.KEY.fst
@@ -1,0 +1,125 @@
+module Setoids.Crypto.KEY
+open FStar.Bytes
+open FStar.UInt32
+open FStar.Map
+open Setoids
+open Setoids.Crypto
+
+module DM = FStar.DependentMap
+////////////////////////////////////////////////////////////////////////////////
+//KEY package
+////////////////////////////////////////////////////////////////////////////////
+
+let handle = h:(bytes&bytes){int_of_bytes (fst h) <= int_of_bytes (snd h)}
+
+let key (n:u32) = lbytes32 n
+let key_state (n:u32) = (Map.t handle (option bool) & Map.t handle (option (key n)))
+
+let key_state_rel (n:u32) = lo (key_state n)
+
+let key_eff (n:u32) = eff (key_state_rel n)
+
+let key_set_t (n:u32) = (lo handle) ** (lo (key n)) ^--> eff_rel (key_state_rel n) (lo handle)
+let key0_set n : key_set_t n =
+    fun (h, k_in) ->
+    s <-- get ;
+    let (h_map,k_map) = s in
+    match Map.sel h_map h,Map.sel k_map h with
+    | None,None ->
+      let s':key_state n = (Map.upd h_map h (Some true), Map.upd k_map h (Some k_in)) in
+      put s' ;;
+      return h
+    | _,_ ->
+      raise
+
+let key1_set n : key_set_t n =
+    fun (h, k_in) ->
+    s <-- get ;
+    let (h_map,k_map) = s in
+    match Map.sel h_map h,Map.sel k_map h with
+    | None,None ->
+      k <-- sample_multiple #(key_state n) n;
+      let s':key_state n = (Map.upd h_map h (Some true), Map.upd k_map h (Some k_in)) in
+      put s' ;;
+      return h
+    | _,_ ->
+      raise
+
+let key_cset_t (n:u32) = (lo handle) ** (lo (key n)) ^--> eff_rel (key_state_rel n) (lo handle)
+let key_cset n : key_cset_t n =
+    fun (h, k_in) ->
+    s <-- get ;
+    let (h_map,k_map) = s in
+    match Map.sel h_map h,Map.sel k_map h with
+    | None, None ->
+      let s':key_state n = (Map.upd h_map h (Some false), Map.upd k_map h (Some k_in)) in
+      put s' ;;
+      return h
+    | _,_ ->
+      raise
+
+let key_get_t (n:u32) = (lo handle) ^--> eff_rel (key_state_rel n) (lo (key n))
+let key_get n : key_get_t n =
+    fun h ->
+    s <-- get ;
+    let (h_map,k_map) = s in
+    match Map.sel h_map h,Map.sel k_map h with
+    | Some hon, Some k ->
+      return k
+    | _,_ ->
+      raise
+
+let key_hon_t (n:u32) = (lo handle) ^--> eff_rel (key_state_rel n) (lo bool)
+let key_hon n : key_hon_t n =
+    fun h ->
+    s <-- get ;
+    let (h_map,k_map) = s in
+    match Map.sel h_map h,Map.sel k_map h with
+    | Some hon, Some k ->
+      return hon
+    | _,_ ->
+      raise
+
+type key_labels =
+  | GET
+  | HON
+  | SET
+  | CSET
+
+let key_field_types n : key_labels -> Type =
+    function  GET -> key_get_t n
+            | HON -> key_hon_t n
+            | SET -> key_set_t n
+            | CSET -> key_cset_t n
+
+let key_field_rels n : (k:key_labels -> erel (key_field_types n k)) =
+  function
+      GET -> arrow (lo handle) (eff_rel (key_state_rel n) (lo (key n)))
+    | HON -> arrow (lo handle) (eff_rel (key_state_rel n) (lo bool))
+    | SET -> arrow (lo handle ** lo (key n)) (eff_rel (key_state_rel n) (lo handle))
+    | CSET -> arrow (lo handle ** lo (key n)) (eff_rel (key_state_rel n) (lo handle))
+
+let key_sig (n:u32) = {
+  labels = key_labels;
+  ops = key_field_types n;
+  rels = key_field_rels n
+  }
+
+let key0_module (n:u32) : module_t (key_sig n) =
+  DM.create #_ #(key_sig n).ops
+    (function GET -> key_get n
+            | HON -> key_hon n
+            | SET -> key0_set n
+            | CSET -> key_cset n)
+
+#set-options "--z3rlimit 350 --max_fuel 2 --max_ifuel 3"
+#set-options "--query_stats"
+let key1_module (n:u32) : module_t (key_sig n) =
+  DM.create #_ #(key_sig n).ops
+    (function GET -> key_get n
+            | HON -> key_hon n
+            | SET -> key1_set n
+            | CSET -> key_cset n)
+
+let key0_functor n = as_fun (key0_module n)
+let key1_functor n = as_fun (key1_module n)
