examples/rel/Setoids.Crypto.ODH.fst
@@ -1,0 +1,89 @@
+module Setoids.Crypto.ODH
+
+open FStar.Bytes
+open FStar.UInt32
+open Setoids
+open Setoids.Crypto
+open Setoids.Crypto.KEY
+
+module DM = FStar.DependentMap
+
+let share (n:u32) = lbytes32 n
+let exponent (n:u32) = lbytes32 n
+assume val exponentiate : #n:u32 -> x:share n -> y:exponent n -> share n
+assume val generator : n:u32 -> lbytes32 n
+
+let odh_state n = Map.t (share n) (option (exponent n))
+
+let gen_dh_t n =
+  (lo unit)
+  ^--> eff_rel (lo (odh_state n) ** lo (key_state n)) (lo (share n))
+let gen_dh n : gen_dh_t n =
+  fun _ ->
+    combined_state  <-- get ;
+    let odh_st = fst combined_state in
+    let key_st = snd combined_state in
+    x_exp <-- sample_multiple #(odh_state n * key_state n) n;
+    let x = exponentiate (generator n) x_exp in
+    let s':odh_state n = Map.upd odh_st x (Some x_exp) in
+    put (s',key_st) ;;
+    return x
+
+/// The key_state relation should be `hi` here.
+let odh_t n =
+  (lo (share n) ** lo (share n))
+  //^--> eff_rel (lo (odh_state n) ** hi (key_state n)) (lo handle)
+  ^--> eff_rel (lo (odh_state n) ** lo (key_state n)) (lo handle)
+
+#reset-options
+#set-options "--z3rlimit 350 --max_fuel 2 --max_ifuel 3"
+#set-options "--query_stats"
+let odh n (key_module:module_t (key_sig n)) : odh_t n =
+  fun (x,y) ->
+    combined_state  <-- get ;
+    let odh_st = fst combined_state in
+    match Map.sel odh_st x with
+    | None ->
+      raise
+    | Some x_exp ->
+      let h =
+        if int_of_bytes x <= int_of_bytes y then
+          (x,y)
+        else
+          (y,x)
+      in
+      let k = exponentiate y x_exp in
+      let k_set : key_set_t n = get_oracle key_module SET in
+      lift_right (k_set (h, k));;
+      return h
+
+type odh_labels =
+  | GEN_DH
+  | ODH
+
+let odh_field_types n : odh_labels -> Type0 =
+  function GEN_DH -> gen_dh_t n
+         | ODH -> odh_t n
+
+let odh_field_rels n : (l:odh_labels -> erel (odh_field_types n l)) =
+  function GEN_DH ->
+           arrow
+             (lo unit)
+             (eff_rel (lo (odh_state n) ** lo (key_state n)) (lo (share n)))
+         | ODH ->
+           arrow
+             (lo (share n) ** lo (share n))
+             (eff_rel (lo (odh_state n) ** lo (key_state n)) (lo handle))
+
+let odh_sig (n:u32) = {
+  labels = odh_labels;
+  ops = odh_field_types n;
+  rels = odh_field_rels n
+  }
+
+let odh_module (n:u32) (km:module_t (key_sig n)) : module_t (odh_sig n) =
+  DM.create #_ #(odh_sig n).ops
+    (function GEN_DH -> gen_dh n
+            | ODH -> odh n km)
+
+//let odh_functor n = as_fun (odh_module n)
